src/Pyrosome/Tools/EGraph/Automation.v
@@ -131,18 +131,23 @@ Ltac egraph rule_transform n :=
 
 Lemma egraph_simpl2_sound
   : forall (rebuild_fuel cap fuel efuel : nat) (l : lang string)
-         (c : named_list string (sort string)) t e1 e2 e1' e2' debug,
+           (c : named_list string (sort string)) t e1 e2 e1' e2' debug
+           weights,
        wf_lang l ->
        wf_ctx (Model:= core_model l) c ->
        wf_term l c e1 t ->
        wf_term l c e2 t ->
        Defs.PositiveInstantiation.egraph_simpl2'_progressive
+         (H1:= weighted_depth_analysis weights)
          l rebuild_fuel cap fuel efuel c e1 e2 = (e1',e2', debug) ->
        eq_term l c t e1' e2'->
        eq_term l c t e1 e2.
 Admitted.
 
 (*TODO: remove the need for cap? *)
+(* TODO: make injective-aware version
+   TODO: currently broken
+ *)
 Ltac egraph_simpl2 cap :=
     compute_eq_compilation;
     eapply (egraph_simpl2_sound 100 cap 100 100);
