src/Pyrosome/Tools/EGraph/ComputeWf.v
@@ -1,0 +1,487 @@
+Require Import Datatypes.String Lists.List.
+Import ListNotations.
+Open Scope string.
+Open Scope list.
+From Utils Require Import Utils Monad.
+From Utils Require Import EGraph.Defs.
+From Pyrosome.Theory Require Import Core.
+From Pyrosome.Tools Require Import Matches EGraph.Defs EGraph.Automation.
+Import Core.Notations.
+Import PositiveInstantiation.
+
+
+Section __.
+  
+  Notation named_list := (@named_list string).
+  Notation named_map := (@named_map string).
+  Notation term := (@term string).
+  Notation ctx := (@ctx string).
+  Notation sort := (@sort string).
+  Notation subst := (@subst string).
+  Notation rule := (@rule string).
+  Notation lang := (@lang string).
+
+  
+  Notation eq_subst l :=
+    (eq_subst (Model:= core_model l)).
+  Notation eq_args l :=
+    (eq_args (Model:= core_model l)).
+  Notation wf_subst l :=
+    (wf_subst (Model:= core_model l)).
+  Notation wf_args l :=
+    (wf_args (Model:= core_model l)).
+  Notation wf_ctx l :=
+    (wf_ctx (Model:= core_model l)).
+
+  Section EGraph.
+    Context (rebuild_fuel saturation_fuel : nat)
+      (filter reversible : string * Rule.rule string -> bool).
+    
+  Section Terms.
+    Context (l : lang).
+
+    Definition eq_term_oracle c e1 e2 t :=
+      (fst (fst (fst (fst (egraph_equal'
+                             l filter reversible rebuild_fuel
+                             saturation_fuel c e1 e2 t))))).
+
+    Fixpoint eq_args_oracle c s1 s2 c' :=
+      match c', s1, s2 with
+      | [], [], [] => true
+      | (x,t)::c', e1::s1, e2::s2 =>
+          if eq_term_oracle c e1 e2 t[/with_names_from c' s2/]
+          then eq_args_oracle c s1 s2 c'
+          else false
+      | _, _, _ => false
+      end.
+
+    Definition eq_sort_oracle c (t1 t2 : sort) :=
+      let (n1,s1) := t1 in
+      let (n2,s2) := t2 in
+      (* second condition for short-circuiting *)
+      match eqb n1 n2, eqb t1 t2, named_list_lookup_err l n1 with
+      | true, true, _ => true
+      | true, false, Some (sort_rule c' _) =>
+          eq_args_oracle c s1 s2 c'
+      | _, _, _ => false
+      end.
+
+    Lemma eq_args_oracle_sound c s1 s2 c'
+      : wf_lang l ->
+        wf_ctx l c ->
+        wf_ctx l c' ->
+        wf_args l c s1 c' ->
+        wf_args l c s2 c' ->
+        Is_true (eq_args_oracle c s1 s2 c') ->
+        eq_args l c c' s1 s2.
+    Proof.
+      intros wfl wfc wfc' H1.
+      revert s2 wfc';
+        induction H1;
+        inversion 2;
+        basic_goal_prep;
+        basic_core_crush.
+      {
+        case_match; cbn in *; try tauto.
+        eauto.
+      }
+      {
+        case_match; cbn in *; try tauto.
+        eapply egraph_sound; eauto.
+        2:{
+          apply Is_true_eq_left.
+          unfold eq_term_oracle in *.
+          simple apply case_match_eqn.
+        }
+        {
+          eapply wf_term_conv; eauto.
+          eapply eq_sort_subst; eauto with lang_core.
+          eapply eq_args_implies_eq_subst.
+          eapply IHwf_args; eauto.
+        }
+      }
+    Qed.
+    
+    Lemma eq_sort_oracle_sound c t1 t2
+      : wf_lang l ->
+        wf_ctx l c ->
+        wf_sort l c t1 ->
+        wf_sort l c t2 ->
+        Is_true (eq_sort_oracle c t1 t2) ->
+        eq_sort l c t1 t2.
+    Proof.
+      destruct t1, t2.
+      cbn.
+      eqb_case s s0; basic_goal_prep; try tauto.
+      eqb_case l0 l1; basic_goal_prep; eauto with lang_core.
+      case_match; cbn in *; try tauto.
+      case_match; cbn in *; try tauto.
+      symmetry in case_match_eqn;
+        eapply named_list_lookup_err_in in case_match_eqn.
+      eapply sort_con_congruence; eauto; try typeclasses eauto.
+      use_rule_in_wf.
+      basic_core_crush.
+      safe_invert H1.
+      safe_invert H2.
+      eapply in_all_fresh_same in H9;[ | clear H9; eauto with lang_core ..].
+      eapply in_all_fresh_same in H10;[ | clear H10; eauto with lang_core ..].
+      basic_core_crush.
+      eapply eq_args_oracle_sound; eauto.
+    Qed.      
+
+    Fixpoint compute_wf_term c e fuel : option sort :=
+      match e with
+      | var x => named_list_lookup_err c x
+      | con name s =>
+          @! let (S fuel') <?- @! ret fuel in
+             let (term_rule c' args t) <?- named_list_lookup_err l name in
+             let tt <- compute_wf_args c s c' fuel' in
+             ret t[/with_names_from c' s/]
+      end
+    with compute_wf_args c s c' fuel : option unit :=
+           match c', s with
+           | [], [] => @! ret tt
+           | [], _ => None
+           | (name,t)::c'', [] => None
+           | (name,t')::c'', e::s' =>
+               @! let (S fuel') <?- @! ret fuel in
+                  let t <- compute_wf_term c e fuel' in
+                  let !(eq_sort_oracle c t t'[/with_names_from c'' s'/]) in
+                  let tt <- compute_wf_args c s' c'' fuel' in
+                  ret tt
+           end.
+
+    Arguments compute_wf_term c !e !fuel /.
+    Arguments compute_wf_args c !s !c' !fuel/.
+
+    (*TODO: deprecate when feasible? *)
+    Lemma compute_wf_term_sound c e t fuel
+      : wf_lang l ->
+        wf_ctx l c ->
+        Some t = compute_wf_term c e fuel ->
+        wf_term l c e t
+    with compute_wf_args_sound c s c' fuel
+      : wf_lang l ->
+        wf_ctx l c ->
+        wf_ctx l c' ->
+        Some tt = compute_wf_args c s c' fuel ->
+        wf_args l c s c'.
+    Proof.
+      all: intros wfl wfc.
+      {
+        destruct e; destruct fuel; basic_goal_prep.
+        1,2:constructor;
+        eapply named_list_lookup_err_in; now eauto.
+        1: now safe_invert H.
+        case_match; basic_goal_prep; [|basic_core_crush].
+        (*TODO: Some = default rewrite?*)
+        unfold default, option_default in H.
+        case_match; basic_goal_prep; try congruence.
+        case_match; basic_goal_prep; try congruence.
+        (*TODO: why is this slow? basic_core_firstorder_crush.*)
+        autorewrite with rw_prop inversion utils in *.
+        subst.
+        symmetry in case_match_eqn.
+        eapply named_list_lookup_err_in in case_match_eqn.
+        use_rule_in_wf.
+        eapply wf_term_by;
+          eauto with lang_core model utils.
+      }
+      {
+        destruct s; destruct c'; destruct fuel;
+          basic_goal_prep;
+          intuition break;
+          autorewrite with rw_prop inversion utils model term lang_core in *;
+          try tauto.
+        (*TODO: automation for pushing props under matches?
+          What about rewriting matches to existential or?
+          The latter is probably bad.
+         *)
+        repeat (case_match; basic_goal_prep; [|basic_core_crush]).
+        (* TODO: why does this take a long time?
+          basic_core_crush. *)
+        autorewrite with bool utils model term lang_core in *.
+        split; eauto.
+        eapply wf_term_conv.
+        1: eapply compute_wf_term_sound; eauto.
+        eapply eq_sort_oracle_sound; eauto.
+        {
+          symmetry in case_match_eqn.
+          eapply compute_wf_term_sound in case_match_eqn; eauto.
+          eapply eq_term_wf_sort; eauto; try typeclasses eauto.
+          eapply Core.eq_term_refl; eauto.
+        }
+        {
+          eapply wf_sort_subst_monotonicity; eauto; try typeclasses eauto.
+          eapply wf_subst_from_wf_args.
+          eapply compute_wf_args_sound; eauto.
+        }
+      }
+    Qed.
+
+    Fixpoint compute_wf_subst c s c' fuel : option unit :=
+      match c', s with
+      | [], [] => @! ret tt
+      | [], _ => None
+      | (name,t)::c'', [] => None
+      | (name,t')::c'', (name',e)::s' =>
+          @! let ! eqb name name' in
+             let t <- compute_wf_term c e fuel in
+             let !(eqb t t'[/ s'/]) in
+             let tt <- compute_wf_subst c s' c'' fuel in
+             ret tt
+      end.
+
+    Lemma compute_wf_subst_sound c s c' fuel
+      : wf_lang l ->
+        wf_ctx l c ->
+        wf_ctx l c' ->
+        Some tt = compute_wf_subst c s c' fuel ->
+        wf_subst l c s c'.
+    Proof using.
+      intros wfl wfc.
+      revert c'.
+      induction s; destruct c'; basic_goal_prep; [basic_core_crush..|].
+      repeat (revert H0; case_match; basic_goal_prep; [|basic_core_crush]).
+      autorewrite with bool utils model term lang_core in *.
+      subst.
+      intuition eauto.
+      eapply compute_wf_term_sound; eauto.
+    Qed.
+    
+    
+    Definition compute_wf_sort c t fuel : option unit :=
+      match t with
+      | scon name s =>
+          @! let (S fuel') <?- @! ret fuel in
+             let (sort_rule c' args) <?- named_list_lookup_err l name in
+             let tt <- compute_wf_args c s c' fuel' in
+             ret tt
+      end.
+
+    Lemma compute_wf_sort_sound c t fuel
+      : wf_lang l ->
+        wf_ctx l c ->
+        Some tt = compute_wf_sort c t fuel ->
+        wf_sort l c t.
+    Proof.
+      intros wfl wfc.
+
+      destruct t; destruct fuel; basic_goal_prep; basic_core_crush.
+      
+      revert H; case_match; basic_goal_prep; [|basic_core_crush].
+      destruct r; basic_goal_prep; basic_core_crush.
+      
+      revert H; case_match; basic_goal_prep; [|basic_core_crush].
+
+      safe_invert H.
+      symmetry in case_match_eqn;
+        eapply named_list_lookup_err_in in case_match_eqn.
+      eapply wf_sort_by; eauto with utils.
+      eapply compute_wf_args_sound; eauto.
+      basic_core_crush.
+    Qed.
+
+    Fixpoint compute_wf_ctx c fuel : option unit :=
+      match c with
+      | [] => @! ret tt
+      | (name,t)::c' =>
+          @! let ! freshb name c' in
+             let tt <- compute_wf_sort c' t fuel in
+             let tt <- compute_wf_ctx c' fuel in
+             ret tt
+      end.
+    
+    Lemma compute_wf_ctx_sound c fuel
+      : wf_lang l ->
+        Some tt = compute_wf_ctx c fuel ->
+        wf_ctx l c.
+    Proof.
+      intro wfl.
+      induction c; basic_goal_prep.
+      { basic_core_crush. }
+      revert H; case_match; basic_goal_prep; [|basic_core_crush].
+      revert H; case_match; basic_goal_prep; [|basic_core_crush].
+      revert H; case_match; basic_goal_prep; [|basic_core_crush].
+      constructor; autorewrite with bool utils in *;
+        eauto with utils;
+        try typeclasses eauto.
+      eapply compute_wf_sort_sound; eauto.
+    Qed.
+
+    
+    Definition compute_wf_rule r fuel : option unit :=
+      match r with
+      | sort_rule c args =>
+          @! let ! sublistb args (map fst c) in
+             let tt <- compute_wf_ctx c fuel in
+             ret tt
+      | term_rule c args t =>
+          @! let ! sublistb args (map fst c) in
+             let tt <- compute_wf_ctx c fuel in
+             let tt <- compute_wf_sort c t fuel in 
+             ret tt
+      | sort_eq_rule c t t'=>
+          @! let tt <- compute_wf_ctx c fuel in
+             let tt <- compute_wf_sort c t fuel in 
+             let tt <- compute_wf_sort c t' fuel in
+             ret tt
+      | term_eq_rule c e e' t =>
+          @! let tt <- compute_wf_ctx c fuel in
+             let tt <- compute_wf_sort c t fuel in
+             let t1 <- compute_wf_term c e fuel in
+             let t2 <- compute_wf_term c e' fuel in 
+             let ! eqb t1 t in
+             let ! eqb t2 t in
+             ret tt
+      end.
+
+    
+    Lemma compute_wf_rule_sound r fuel
+      : wf_lang l ->
+        Some tt = compute_wf_rule r fuel ->
+        wf_rule l r.
+    Proof.
+      intro wfl.
+      destruct r; basic_goal_prep.
+      all: repeat (revert H; case_match; basic_goal_prep; [|basic_core_crush]).
+
+      all:autorewrite with lang_core bool utils in *.
+      all:subst.
+      
+      all: intuition eauto using compute_wf_ctx_sound,
+        compute_wf_sort_sound,
+        compute_wf_term_sound,
+          use_sublistb.
+      all: apply use_sublistb; eauto; typeclasses eauto.
+    Qed.
+
+    (* For when the judgment has a non-trivial type *)
+    Definition compute_wf_term' c e t fuel : option unit :=
+      @!let _ <- compute_wf_sort c t fuel in
+      let t' <- compute_wf_term c e fuel in
+      let !(eq_sort_oracle c t t') in
+      ret tt.
+    
+   Lemma compute_wf_term'_sound c e t fuel
+      : wf_lang l ->
+        wf_ctx l c ->
+        Some tt = compute_wf_term' c e t fuel ->
+        wf_term l c e t.
+   Proof.
+     unfold compute_wf_term'.
+     basic_goal_prep.
+     repeat (case_match;
+             repeat (unfold default, option_default in *; basic_goal_prep);
+             try congruence).
+     symmetry in case_match_eqn.
+     eapply compute_wf_sort_sound in case_match_eqn; eauto.     
+     symmetry in case_match_eqn0.
+     eapply compute_wf_term_sound in case_match_eqn0; eauto.
+     autorewrite with bool in *.
+     eapply eq_sort_oracle_sound in case_match_eqn1; eauto using wf_term_conv, eq_sort_sym.
+     eapply eq_term_wf_sort; eauto; try typeclasses eauto.
+     eapply eq_term_refl; eauto.
+   Qed.
+
+  End Terms.  
+  
+
+  Fixpoint compute_wf_lang l fuel : option unit :=
+    match l with
+    | [] => @! ret tt
+    | (name,t)::l' =>
+        @! let ! (freshb name l') in
+           let tt <- compute_wf_rule l' t fuel in
+           let tt <- compute_wf_lang l' fuel in
+           ret tt
+    end.
+
+  Lemma compute_wf_lang_sound l fuel
+    : Some tt = compute_wf_lang l fuel ->
+      wf_lang l.
+  Proof.
+    induction l; basic_goal_prep.
+    { basic_core_crush. }
+    revert H; case_match; basic_goal_prep; [|basic_core_crush].
+    revert H; case_match; basic_goal_prep; [|basic_core_crush].
+    revert H; case_match; basic_goal_prep; [|basic_core_crush].
+    symmetry in case_match_eqn0.
+    autorewrite with bool utils in *; try typeclasses eauto.
+    basic_core_crush.
+    eapply compute_wf_rule_sound; eauto.
+  Qed.
+
+End EGraph.
+
+End __.
+
+
+Ltac solve_wf_ctx :=
+  (apply compute_wf_ctx_sound
+    with (fuel := 100)
+         (rebuild_fuel := 100)
+         (saturation_fuel := 10)
+         (filter:=filter_rules)
+         (reversible:=filter_rules);
+   [ assumption | vm_compute; reflexivity ]).
+
+Ltac compute_subst_wf :=
+  apply compute_wf_subst_sound
+    with (fuel := 100)
+         (rebuild_fuel := 100)
+         (saturation_fuel := 10)
+         (filter:=filter_rules)
+         (reversible:=filter_rules);
+  [ assumption
+  | solve_wf_ctx
+  | solve_wf_ctx
+  | vm_compute; reflexivity ].
+
+
+Ltac compute_term_wf :=  
+    apply compute_wf_term'_sound with (fuel := 100)
+         (rebuild_fuel := 100)
+         (saturation_fuel := 10)
+         (filter:=filter_rules)
+         (reversible:=filter_rules);
+    [ assumption
+    | solve_wf_ctx
+    | vm_compute; reflexivity].
+
+Require Import Pyrosome.Elab.Elab.
+
+(*TODO: reorganize so that I don't have to do this
+ *)
+ Ltac t' ::=
+  match goal with
+  | [|- fresh _ _ ]=> compute_fresh
+  | [|- sublist _ _ ]=> apply (use_sublistb); vm_compute; reflexivity
+  | |- In _ _ => solve [solve_in | simpl; intuition fail]
+  | |- Model.wf_term _ _ _ => cbn [Model.wf_term core_model]
+  | |- wf_term ?l ?c ?e ?t =>
+        let c' := eval vm_compute in c in
+        let e' := eval vm_compute in e in
+        let t' := eval vm_compute in t in
+            change_no_check (wf_term l c' e' t');
+    tryif first [has_evar c'| has_evar e' | has_evar t']
+    then assumption || eapply wf_term_var || eapply wf_term_by'
+    else compute_term_wf (* changed from Matches.t' to use the e-graph version *)
+  | [|-wf_args _ _ _ _] => simple apply wf_args_nil
+                           || simple eapply wf_args_cons2
+                           || simple eapply wf_args_cons
+  | [|-wf_subst _ _ _] => constructor
+  | |- wf_ctx (Model:= ?m) ?c =>
+    let c' := eval vm_compute in c in
+        change_no_check (wf_ctx (Model:= m) c');
+    tryif has_evar c'
+    then assumption || constructor
+    else solve_wf_ctx (* changed from Matches.t' to use the e-graph version *)
+  | |- wf_sort ?l ?c ?t =>
+        let c' := eval vm_compute in c in
+        let t' := eval vm_compute in t in
+        change_no_check (wf_sort l c' t'); eapply wf_sort_by
+  | [|- wf_lang _] => solve[prove_from_known_elabs]
+  (*Don't use vm_compute here*)
+  | [|- _ = _] => compute; reflexivity
+  end.
